Validator/Regex/Memoize/Leave.lean
@@ -4,37 +4,37 @@ import Validator.Std.Memoize
 import Validator.Regex.Regex
 import Validator.Regex.Leave
 
-namespace Regex
+namespace Regex.Memoize
 
 abbrev leaveParam (σ: Type) := Σ (r: Regex σ), (Vector Bool (symbols r))
 abbrev leaveResult {σ: Type} (_: leaveParam σ) := Regex σ
 
-def leave2 {σ: Type}: (a: leaveParam σ) → leaveResult a
-  | ⟨r, bools⟩ => leave r bools
+def leave {σ: Type}: (a: leaveParam σ) → leaveResult a
+  | ⟨r, bools⟩ => Regex.leave r bools
 
-abbrev leaveMemTable (σ: Type) [DecidableEq σ] [Hashable σ] := MemTable leave2 (α := leaveParam σ)
+abbrev leaveMemTable (σ: Type) [DecidableEq σ] [Hashable σ] := MemTable leave (α := leaveParam σ)
 
-def MemTable.leaveM {σ: Type} [DecidableEq σ] [Hashable σ] [Monad m] [monadState: MonadState (leaveMemTable σ) m]
-  (param: leaveParam σ): m { res // res = leave2 param } :=
-  MemTable.call leave2 param
+def MemTable.leave {σ: Type} [DecidableEq σ] [Hashable σ] [Monad m] [monadState: MonadState (leaveMemTable σ) m]
+  (param: leaveParam σ): m { res // res = Regex.Memoize.leave param } :=
+  MemTable.call Regex.Memoize.leave param
 
 private theorem MemTable.leaveM_is_correct [DecidableEq σ] [Hashable σ] (param: leaveParam σ) (table: leaveMemTable σ):
-  leave2 param = (StateM.run (s := table) (leaveM param)).1 := by
-  generalize (StateM.run (leaveM param) table) = x
+  Regex.Memoize.leave param = (StateM.run (s := table) (leave param)).1 := by
+  generalize (StateM.run (leave param) table) = x
   obtain ⟨⟨res, hres⟩, table'⟩ := x
   simp only
   rw [hres]
 
 instance {σ: Type} [DecidableEq σ] [Hashable σ] [Monad m] [MonadState (leaveMemTable σ) m]:
-  Memoize (α := leaveParam σ) (β := leaveResult) leave2 m where
-  call param := MemTable.leaveM param
+  Memoize (α := leaveParam σ) (β := leaveResult) Regex.Memoize.leave m where
+  call param := MemTable.leave param
 
-abbrev MemoizedLeave (σ: Type) [DecidableEq σ] [Hashable σ] := Memoize (@leave2 σ) (StateM (leaveMemTable σ))
+abbrev MemoizedLeave (σ: Type) [DecidableEq σ] [Hashable σ] := Memoize (@Regex.Memoize.leave σ) (StateM (leaveMemTable σ))
 
 private theorem Memoize.StateM.leaveM_is_correct
   [DecidableEq σ] [Hashable σ] [memleave: MemoizedLeave σ]
   (param: leaveParam σ) (table: leaveMemTable σ):
-  leave2 param = (memleave.call param table).1 := by
+  Regex.Memoize.leave param = (memleave.call param table).1 := by
   generalize (memleave.call param table) = x
   obtain ⟨⟨res, hres⟩, table'⟩ := x
   simp only
