Validator/Regex/Memoize/Memoize.lean
@@ -12,52 +12,53 @@ import Validator.Regex.Room
 import Validator.Regex.Memoize.Enter
 import Validator.Regex.Memoize.Leave
 
-namespace Regex
+namespace Regex.Memoize
 
 class MemoizeRoom (m: Type -> Type u) (σ: Type) [DecidableEq σ] [Hashable σ] where
   enterM : (a: enterParam σ) -> m { b: enterResult a // b = enter a }
-  leaveM : (a: leaveParam σ) -> m { b: leaveResult a // b = leave2 a }
+  leaveM : (a: leaveParam σ) -> m { b: leaveResult a // b = leave a }
 
 instance (m: Type -> Type u) (σ: Type) [DecidableEq σ] [Hashable σ] [Monad m]
   [DecidableEq (enterParam σ)] [Hashable (enterParam σ)]
   [Memoize (α := enterParam σ) (β := enterResult) enter m]
   [enterState: MonadState (enterMemTable σ) m]
   [DecidableEq (leaveParam σ)] [Hashable (leaveParam σ)]
-  [Memoize (α := leaveParam σ) (β := leaveResult) leave2 m]
+  [Memoize (α := leaveParam σ) (β := leaveResult) leave m]
   [leaveState: MonadState (leaveMemTable σ) m]
   : MemoizeRoom m σ where
-  enterM param := MemTable.enterM (monadState := enterState) param
-  leaveM param := MemTable.leaveM (monadState := leaveState) param
+  enterM param := MemTable.enter (monadState := enterState) param
+  leaveM param := MemTable.leave (monadState := leaveState) param
 
-end Regex
-
-def Regex.Mem.derive [Monad m] [DecidableEq σ] [Hashable σ] [MemoizeRoom m σ]
+def derive [Monad m] [DecidableEq σ] [Hashable σ] [MemoizeRoom m σ]
   (Φ: σ → Bool) (r: Regex σ): m {dr: Regex σ // dr = Regex.Room.derive Φ r } := do
   let ⟨ifexpr, hifexpr⟩ <- MemoizeRoom.enterM r
   let ⟨res, hres⟩ <- MemoizeRoom.leaveM ⟨r, IfExpr.eval Φ ifexpr⟩
   let h: res = r.leave (IfExpr.eval Φ r.enter) := by
-    unfold leave2 at hres
+    unfold leave at hres
     simp only at hres
     rw [hifexpr] at hres
     assumption
   pure (Subtype.mk res h)
 
-private def Regex.Mem.StateM.derive [DecidableEq σ] [Hashable σ] (Φ: σ → Bool) (r: Regex σ)
+private def StateM.derive [DecidableEq σ] [Hashable σ] (Φ: σ → Bool) (r: Regex σ)
   : StateT (enterMemTable σ) (StateM (leaveMemTable σ)) (Regex σ) :=
-  Regex.Mem.derive Φ r
+  Regex.Memoize.derive Φ r
 
-private def Regex.Mem.StateM.derive.run [DecidableEq σ] [Hashable σ] (Φ: σ → Bool) (r: Regex σ)
-  (enterState: Regex.enterMemTable σ) (leaveState: Regex.leaveMemTable σ): Regex σ :=
-  ((StateM.run (StateT.run (Regex.Mem.derive Φ r) enterState) leaveState).1).1
+private def StateM.derive.run [DecidableEq σ] [Hashable σ]
+  (enterState: enterMemTable σ) (leaveState: leaveMemTable σ)
+  (Φ: σ → Bool) (r: Regex σ): Regex σ :=
+  ((StateM.run (StateT.run (Regex.Memoize.derive Φ r) enterState) leaveState).1).1
 
-theorem run_is_correct [DecidableEq σ] [Hashable σ] (Φ: σ → Bool) (r: Regex σ)
-  (enterState: Regex.enterMemTable σ) (leaveState: Regex.leaveMemTable σ):
-  Regex.Mem.StateM.derive.run Φ r enterState leaveState = Regex.Room.derive Φ r := by
-  unfold Regex.Mem.StateM.derive.run
-  generalize ((StateM.run (StateT.run (Regex.Mem.derive Φ r) enterState) leaveState)).1.1 = x
+theorem run_is_correct [DecidableEq σ] [Hashable σ]
+  (enterState: enterMemTable σ) (leaveState: leaveMemTable σ)
+  (Φ: σ → Bool) (r: Regex σ):
+  StateM.derive.run enterState leaveState Φ r = Regex.Room.derive Φ r := by
+  unfold StateM.derive.run
+  generalize ((StateM.run (StateT.run (Regex.Memoize.derive Φ r) enterState) leaveState)).1.1 = x
   obtain ⟨dr, hdr⟩ := x
   simp only
   rw [hdr]
 
-#guard Regex.Mem.StateM.derive.run (· == 'a') (Regex.or (Regex.symbol 'a') (Regex.symbol 'b')) (MemTable.init Regex.enter) (MemTable.init Regex.leave2)
+#guard StateM.derive.run (MemTable.init enter) (MemTable.init leave)
+  (· == 'a') (Regex.or (Regex.symbol 'a') (Regex.symbol 'b'))
   = Regex.or Regex.emptystr Regex.emptyset
